proof of theorem complete assuming inveresion lemmas

coq/two/LambdaTwo.v
@@ -2,48 +2,42 @@ Require Export LambdaTwoSyntax.
 Require Export IndistinguishabilityTwo.
 Require Import LibTactics.
 
-Fixpoint eval (L : two) (P : value -> value -> Prop) (pc : two) (e : env)
-         (t : term) (k : nat) (a : atom) {struct k} :=
-  match t with
-    | TNat n =>
+Fixpoint eval (L : two) (P : value -> value -> Prop)
+         (pc : two) (e : env) (t : term) (k : nat) (a : atom)
+         {struct k} : Prop :=
+  match t, k with
+    | TNat n, 0 =>
       a = Atom (VNat n) pc
-    | TVar n =>
+    | TVar n, 0 =>
       match atIndex e n with
         | Some (Atom v l) =>
           a = Atom v (l ⊔ pc)
         | None => False
       end
-    | TAbs t' =>
+    | TAbs t', 0 =>
       a = Atom (VClos e t') pc
-    | TApp t1 t2 =>
-      match k with
-        | S k' =>
-          forall e1' t1' l1 a2 a3,
-            eval L P pc e t1 k' (Atom (VClos e1' t1') l1) ->
-            eval L P pc e t2 k' a2 ->
-            eval L P l1 (a2 :: e1') t1' k' a3 ->
-            a = a3
-        | 0 => False
-      end
-    | TDecl t1 t2 =>
-      match k with
-        | S k' =>
-          forall e1' t1' l1 a2 v3 l3,
-            eval L P pc e t1 k' (Atom (VClos e1' t1') l1) ->
-            eval L P pc e t2 k' a2 ->
-            eval L P l1 (a2 :: e1') t1' k' (Atom v3 l3) ->
-            match l3 with
-              | Bottom2 =>
-                a = Atom v3 Bottom2
-              | Top2 =>
-                (forall a2' e2' v3',
-                   env_LPequiv L P (a2 :: e1') (a2' :: e2') ->
-                   eval L P l1 (a2' :: e2') t1' k' (Atom v3' Top2) ->
-                   value_LPequiv L P v3 v3') ->
-                a = Atom v3 Bottom2
-            end
-        | 0 => False
-      end
+    | TApp t1 t2, S k' =>
+      forall e1' t1' l1 a2 a3,
+        eval L P pc e t1 k' (Atom (VClos e1' t1') l1) ->
+        eval L P pc e t2 k' a2 ->
+        eval L P l1 (a2 :: e1') t1' k' a3 ->
+        a = a3
+    | TDecl t1 t2, S k' =>
+      forall e1' t1' l1 a2 v3 l3,
+        eval L P pc e t1 k' (Atom (VClos e1' t1') l1) ->
+        eval L P pc e t2 k' a2 ->
+        eval L P l1 (a2 :: e1') t1' k' (Atom v3 l3) ->
+        match l3 with
+          | Bottom2 =>
+            a = Atom v3 Bottom2
+          | Top2 =>
+            (forall a2' e2' v3',
+               env_LPequiv L P (a2 :: e1') (a2' :: e2') ->
+               eval L P l1 (a2' :: e2') t1' k' (Atom v3' Top2) ->
+               value_LPequiv L P v3 v3') ->
+            a = Atom v3 Bottom2
+        end
+    | _, _ => False
   end.
 
 Lemma eval_nat_inv :
@@ -51,51 +45,55 @@ Lemma eval_nat_inv :
     eval L P pc e (TNat n) k a ->
     a = Atom (VNat n) pc.
 Proof.
-  introv Heval.
-  destruct k; auto.
+  introv Heval. destruct k; auto.
 Qed.
 
 Lemma eval_var_inv :
-  forall L P k pc e n v l a,
+  forall L P k pc e n a,
     eval L P pc e (TVar n) k a ->
-    a = Atom v l ->
-    (l = Bottom2 /\
-     atIndex e n = Some (Atom v Bottom2)) \/
-    (l = Top2 /\ pc = Top2 /\
-     atIndex e n = Some (Atom v Bottom2)) \/
-    (l = Top2 /\ pc = Top2 /\
-     atIndex e n = Some (Atom v Top2)) \/
-    (l = Top2 /\ pc = Bottom2 /\
-     atIndex e n = Some (Atom v Top2)).
+    exists v l,
+      atIndex e n = Some (Atom v l) /\
+      a = Atom v (l ⊔ pc).
 Proof.
-  introv Heval Ha.
-  destruct l; destruct pc; subst.
-  - destruct k; unfold eval in Heval;
-    remember (atIndex e n) as o; destruct o as [[v' l'] |]; subst; auto;
-    rewrite join_bot in Heval; inversion Heval;
-    left; auto.
-  - destruct k; unfold eval in Heval;
-    remember (atIndex e n) as o; destruct o as [[v' l'] |]; subst; auto;
-    rewrite join_top in Heval; inversion Heval; 
-    left; auto.
-  - destruct k; unfold eval in Heval;
-    remember (atIndex e n) as o; destruct o as [[v' l'] |]; subst; auto;
-    rewrite join_bot in Heval; inversion Heval;
-    right; right; right; auto.
-  - destruct k; unfold eval in Heval;
-    remember (atIndex e n) as o; destruct o as [[v' l'] |]; subst; auto;
-    inversion Heval; destruct l'.
-    + right. left. auto.
-    + right. right. left. auto.
-    + right. left. auto.
-    + right. right. left. auto.
+  introv Heval. remember (atIndex e n) as o.
+  destruct o as [[v' l'] |]; destruct pc; destruct k;
+  unfold eval in Heval; try rewrite <- Heqo in Heval; inversion Heval;
+  apply ex_intro with v'; apply ex_intro with l'; auto.
 Qed.
-
+               
 Lemma eval_abs_inv :
   forall L P k pc e t a,
     eval L P pc e (TAbs t) k a ->
     a = Atom (VClos e t) pc.
 Proof.
-  introv Heval.
-  destruct k; auto.
+  introv Heval. destruct k; auto.
 Qed.
+
+Lemma eval_app_inv :
+  forall L P k' pc e t1 t2 a,
+    eval L P pc e (TApp t1 t2) (S k') a ->
+    exists e1' t1' l1 a2 a3,
+      eval L P pc e t1 k' (Atom (VClos e1' t1') l1) /\
+      eval L P pc e t2 k' a2 /\
+      eval L P l1 (a2 :: e1') t1' k' a3 /\
+      a = a3.
+Proof.
+  Admitted.
+
+Lemma eval_decl_inv :
+  forall L P k' pc e t1 t2 a,
+    eval L P pc e (TDecl t1 t2) (S k') a ->
+    exists e1' t1' l1 a2 v3 l3,
+      eval L P pc e t1 k' (Atom (VClos e1' t1') l1) /\
+      eval L P pc e t2 k' a2 /\
+      eval L P l1 (a2 :: e1') t1' k' (Atom v3 l3) /\
+      (l3 = Bottom2 /\
+       a = Atom v3 Bottom2 \/
+       l3 = Top2 /\
+       (forall a2' e2' v3',
+          env_LPequiv L P (a2 :: e1') (a2' :: e2') ->
+          eval L P l1 (a2' :: e2') t1' k' (Atom v3' Top2) ->
+          value_LPequiv L P v3 v3') /\
+       a = Atom v3 Bottom2).
+Proof.
+  Admitted.
